work

Wavelet/Call.lean
@@ -12,28 +12,31 @@ structure Sig where
   ι : Nat
   ω : Nat
 
-/-- TODO: can't refer to the last signature? -/
-inductive SigOps (sigs : Vector Sig k) (k' : Fin k) where
+inductive SigOps (sigs : Vector Sig k) (k' : Fin (k + 1)) where
   | call (i : Fin k')
   deriving DecidableEq
 
-def SigOps.toFin {k' : Fin k} : SigOps sigs k' → Fin k'
+def SigOps.toFin {k' : Fin (k + 1)} : SigOps sigs k' → Fin k'
   | .call i => i
 
-def SigOps.elim0 {hlt : 0 < k} : SigOps sigs ⟨0, hlt⟩ → α
+def SigOps.elim0 : SigOps sigs ⟨0, by simp⟩ → α
   | .call i => i.elim0
 
 instance : Arity (SigOps sigs k') where
   ι | .call i => sigs[i].ι
   ω | .call i => sigs[i].ω
 
-abbrev Prog (Op : Type u) χ {k} [Arity Op] (sigs : Vector Sig k) :=
-  (i : Fin k) → Fn (Op ⊕ SigOps sigs i) χ sigs[i].ι sigs[i].ω
+abbrev Prog (Op : Type u) χ V [Arity Op] (sigs : Vector Sig k) :=
+  (i : Fin k) → Fn (Op ⊕ SigOps sigs i.castSucc) χ V sigs[i].ι sigs[i].ω
+
+/-- A list of `Proc`s with each being able to call previous `Proc`s. -/
+abbrev DepProcs (Op : Type u) χ V [Arity Op] (sigs : Vector Sig k) :=
+  (i : Fin k) → Proc (Op ⊕ SigOps sigs i.castSucc) χ V sigs[i].ι sigs[i].ω
 
 def Prog.semantics
   [Arity Op] [DecidableEq χ] [InterpConsts V]
   {sigs : Vector Sig k}
-  (prog : Prog Op χ sigs)
+  (prog : Prog Op χ V sigs)
   : (i : Fin k) → Semantics Op V sigs[i].ι sigs[i].ω
   -- Nothing more to interpret
   | ⟨0, hlt⟩ => (prog ⟨0, hlt⟩).semantics.link (·.elim0)
@@ -41,5 +44,233 @@ def Prog.semantics
   | ⟨i + 1, hlt⟩ =>
     (prog ⟨i + 1, hlt⟩).semantics.link
       (λ op => Prog.semantics prog ⟨op.toFin, by omega⟩)
+
+def DepProcs.semantics
+  [Arity Op] [DecidableEq χ] [InterpConsts V]
+  {sigs : Vector Sig k}
+  (deps : DepProcs Op χ V sigs)
+  : (i : Fin k) → Semantics Op V sigs[i].ι sigs[i].ω
+  | ⟨0, hlt⟩ => (deps ⟨0, hlt⟩).semantics.link (·.elim0)
+  | ⟨i + 1, hlt⟩ =>
+    (deps ⟨i + 1, hlt⟩).semantics.link
+      (λ op => DepProcs.semantics deps ⟨op.toFin, by omega⟩)
+
+/-- Channel name prefixes to disambiguate names during linking. -/
+inductive LinkName (χ : Type u) where
+  | base (name : χ)
+  | main (name : LinkName χ)
+  | dep (i : Nat) (name : LinkName χ)
+
+/-- TODO: should be auto-derived -/
+instance [inst : DecidableEq χ] : DecidableEq (LinkName χ) := sorry
+
+def linkAtomicProc
+  [Arity Op]
+  (sigs : Vector Sig k)
+  (k' : Fin (k + 1))
+  (procs : (i : Fin k') → Proc Op (LinkName χ) V sigs[i].ι sigs[i].ω)
+  (idx : Nat) -- Index of the atomic proc
+  (atom : AtomicProc (Op ⊕ (SigOps sigs k')) (LinkName χ) V)
+  : AtomicProcs Op (LinkName χ) V :=
+  match atom with
+  | .op (.inl o) inputs outputs =>
+    [.op o (inputs.map .main) (outputs.map .main)]
+  | .op (.inr (.call i)) inputs outputs =>
+    [ .forward (inputs.map .main) ((procs i).inputs.map (LinkName.dep idx)) ] ++
+    (procs i).atoms.mapChans (LinkName.dep idx) ++
+    [ .forward ((procs i).outputs.map (LinkName.dep idx)) (outputs.map .main) ]
+  | .switch decider inputs outputs₁ outputs₂ =>
+    [.switch (.main decider) (inputs.map .main) (outputs₁.map .main) (outputs₂.map .main)]
+  | .steer flavor decider inputs outputs =>
+    [.steer flavor (.main decider) (inputs.map .main) (outputs.map .main)]
+  | .carry inLoop decider inputs₁ inputs₂ outputs =>
+    [.carry inLoop (.main decider) (inputs₁.map .main) (inputs₂.map .main) (outputs.map .main)]
+  | .merge decider inputs₁ inputs₂ outputs =>
+    [.merge (.main decider) (inputs₁.map .main) (inputs₂.map .main) (outputs.map .main)]
+  | .forward inputs outputs => [.forward (inputs.map .main) (outputs.map .main)]
+  | .fork input outputs => [.fork (.main input) (outputs.map .main)]
+  | .const c act outputs => [.const c act (outputs.map .main)]
+  | .forwardc inputs consts outputs => [.forwardc (inputs.map .main) consts (outputs.map .main)]
+  | .sink inputs => [.sink (inputs.map .main)]
+
+/-- Inline calls to the given `k` processes while preserving a forward simulation. -/
+def linkProcs
+  [Arity Op]
+  (sigs : Vector Sig k)
+  (k' : Fin (k + 1))
+  (procs : (i : Fin k') → Proc Op (LinkName χ) V sigs[i].ι sigs[i].ω)
+  (main : Proc (Op ⊕ SigOps sigs k') (LinkName χ) V m n)
+  : Proc Op (LinkName χ) V m n := {
+    inputs := main.inputs.map LinkName.main,
+    outputs := main.outputs.map LinkName.main,
+    atoms := (main.atoms.mapIdx (linkAtomicProc sigs k' procs)).flatten,
+  }
+
+/-- Given a program (a list of functions that non-recursively call each other),
+compile the `i`-th function to a process without any dependencies. -/
+def compileProg
+  [Arity Op] [DecidableEq χ] [InterpConsts V]
+  (sigs : Vector Sig k)
+  (prog : Prog Op χ V sigs)
+  (hnz : ∀ i : Fin k, sigs[i].ι > 0 ∧ sigs[i].ω > 0)
+  (i : Fin k) : Proc Op (LinkName (ChanName χ)) V sigs[i].ι sigs[i].ω :=
+  -- Compile the current function
+  let proc : Proc (Op ⊕ SigOps sigs i.castSucc) (LinkName (ChanName χ)) V _ _ :=
+    compileFn (by apply hnz) (prog i) |>.mapChans LinkName.base
+  -- Compile dependencies
+  let deps : (j : Fin i) → Proc Op (LinkName (ChanName χ)) V sigs[j].ι sigs[j].ω :=
+    λ j => compileProg sigs prog hnz (j.castLT (by omega))
+  -- Link everything into one dataflow graph
+  linkProcs sigs i.castSucc deps proc
+
+/-- TODO: Migrate the proofs of the older version over. -/
+theorem sim_compile_fn
+  [Arity Op]
+  [InterpConsts V]
+  [DecidableEq χ]
+  (hnz : m > 0 ∧ n > 0)
+  (fn : Fn Op χ V m n)
+  (hwf : fn.WellFormed) :
+  fn.semantics ∼ (compileFn hnz fn).semantics
+  := sorry
+
+theorem sim_congr_link
+  [Arity Op₀] [Arity Op₁]
+  [DecidableEq Op₁]
+  {main main' : Semantics (Op₀ ⊕ Op₁) V m n}
+  {deps deps' : PartInterp Op₀ Op₁ V}
+  (hsim_deps : ∀ i, deps i ∼ deps' i)
+  (hsim_main : main ∼ main')
+  : main.link deps ∼ main'.link deps'
+  := sorry
+
+def Expr.castWithSigs0
+  [Arity Op]
+  {sigs : Vector Sig k}
+  (hz : ↑i = 0) :
+  Expr (Op ⊕ SigOps sigs i) χ m n → Expr Op χ m n
+  | .ret vars => .ret vars
+  | .tail vars => .tail vars
+  | .op (.inl o) inputs outputs cont =>
+    .op o inputs outputs (castWithSigs0 hz cont)
+  | .op (.inr (.call f)) .. => by
+    simp [hz] at f
+    exact f.elim0
+  | .br cond left right => .br cond (castWithSigs0 hz left) (castWithSigs0 hz right)
+
+def Fn.castWithSigs0
+  [Arity Op]
+  {sigs : Vector Sig k}
+  (hz : ↑i = 0)
+  (fn : Fn (Op ⊕ SigOps sigs i) χ V m n) :
+  Fn Op χ V m n := {
+    params := fn.params,
+    body := Expr.castWithSigs0 hz fn.body,
+  }
+
+def AtomicProc.castWithSigs0
+  [Arity Op]
+  {sigs : Vector Sig k}
+  (hz : ↑i = 0)
+  : AtomicProc (Op ⊕ SigOps sigs i) χ V → AtomicProc Op χ V
+  | _ => sorry
+
+def Proc.castWithSigs0
+  [Arity Op]
+  {sigs : Vector Sig k}
+  (hz : ↑i = 0)
+  (proc : Proc (Op ⊕ SigOps sigs i) χ V m n)
+  : Proc Op χ V m n := {
+    inputs := proc.inputs,
+    outputs := proc.outputs,
+    atoms := proc.atoms.map (AtomicProc.castWithSigs0 hz),
+  }
+
+/-- Linking without dependencies is the same as renaming the channels. -/
+def link_procs_0_eq_renaming
+  [Arity Op]
+  {sigs : Vector Sig k}
+  {i : Fin (k + 1)}
+  (hz : ↑i = 0)
+  {deps : (j : Fin ↑i) → Proc Op (LinkName χ) V sigs[j].ι sigs[j].ω}
+  {proc : Proc (Op ⊕ SigOps sigs i) (LinkName χ) V m n} :
+  linkProcs sigs i deps proc
+  = (Proc.castWithSigs0 hz proc).mapChans LinkName.main := sorry
+
+/-- `Proc.castWithSigs0` commutes with `Proc.mapChans`. -/
+def proc_cast_sigs_0_comm_map_chans
+  [Arity Op]
+  {sigs : Vector Sig k}
+  {f : χ → χ'}
+  {i : Fin (k + 1)}
+  (hz : ↑i = 0)
+  (proc : Proc (Op ⊕ SigOps sigs i) χ V m n) :
+  Proc.castWithSigs0 hz (proc.mapChans f)
+  = (Proc.castWithSigs0 hz proc).mapChans f := sorry
+
+def sim_proc_cast_sigs_0_semantics_link
+  [Arity Op]
+  [DecidableEq χ]
+  [InterpConsts V]
+  {sigs : Vector Sig k}
+  {i : Fin (k + 1)}
+  {deps : PartInterp Op (SigOps sigs i) V}
+  {proc : Proc (Op ⊕ SigOps sigs i) χ V m n}
+  (hz : ↑i = 0) :
+  proc.semantics.link deps ∼
+  (Proc.castWithSigs0 hz proc).semantics := sorry
+
+theorem sim_map_chans_inj
+  {χ χ' : Type u}
+  [Arity Op]
+  [DecidableEq χ]
+  [DecidableEq χ']
+  [InterpConsts V]
+  {f : χ → χ'}
+  {proc : Proc Op χ V m n}
+  (hf : Function.Injective f) :
+  proc.semantics ∼ (proc.mapChans f).semantics := sorry
+
+-- theorem sim_proc_cast_sigs_0
+--   [Arity Op]
+--   [DecidableEq χ]
+--   [InterpConsts V]
+--   {sigs : Vector Sig k}
+--   {i : Fin (k + 1)}
+--   (hz : ↑i = 0)
+--   (proc : Proc (Op ⊕ SigOps sigs i) χ V m n) :
+--   (Proc.castWithSigs0 hz proc).semantics (χ := χ) ∼ proc.semantics
+--   := sorry
+
+theorem sim_compile_prog
+  {Op : Type u} {χ : Type v} {V : Type w}
+  [Arity Op]
+  [InterpConsts V]
+  [DecidableEq χ]
+  (sigs : Vector Sig k)
+  (prog : Prog Op χ V sigs)
+  (i : Fin k)
+  (hnz : ∀ (i : Fin k), sigs[i].ι > 0 ∧ sigs[i].ω > 0)
+  (hwf : ∀ i, (prog i).WellFormed) :
+  prog.semantics i ∼ (compileProg sigs prog hnz i).semantics
+  := by
+  have ⟨i', hlt⟩ := i
+  induction i' with
+  | zero =>
+    simp [Prog.semantics]
+    unfold compileProg
+    rw [link_procs_0_eq_renaming (by simp)]
+    rw [← proc_cast_sigs_0_comm_map_chans]
+    apply Semantics.SimilarBy.trans _
+      (sim_proc_cast_sigs_0_semantics_link (deps := λ x => x.elim0) (by simp))
+    apply sim_congr_link.{_, _, _, _, _, _, u} -- TODO: avoid this explicit universe annotation
+    · intros i
+      exact i.elim0
+    · apply Semantics.SimilarBy.trans _
+        (sim_map_chans_inj (by simp [Function.Injective]))
+      apply Semantics.SimilarBy.trans _
+        (sim_map_chans_inj (by simp [Function.Injective]))
+      apply sim_compile_fn _ _ (by apply hwf)
+  | succ => sorry
 
 end Wavelet.Call
