Wavelet/LTS.lean
@@ -43,17 +43,57 @@ inductive LTS.Star (R : Lts C E) : Lts C (Trace E) where
   | refl : Star R c .ε c
   | tail : Star R c tr c' → R c' tr' c'' → Star R c (.cons tr tr') c''
 
-structure Lts.Simulates
+structure Lts.SimulatedBy
   (lts₁ : Lts C₁ E)
   (lts₂ : Lts C₂ E)
   (R : C₁ → C₂ → Prop)
   (c₁ : C₁) (c₂ : C₂) : Prop where
   init : R c₁ c₂
-  coind : ∀ c₁ l c₁',
+  coind : ∀ c₁ c₂ l c₁',
     R c₁ c₂ →
     lts₁.Step c₁ l c₁' →
     ∃ c₂',
       lts₂.Step c₂ l c₂' ∧
       R c₁' c₂'
+
+inductive Lts.SimilarBy
+  (lts₁ : Lts C₁ E)
+  (lts₂ : Lts C₂ E)
+  (c₁ : C₁) (c₂ : C₂) : Prop where
+  | mk (Sim : C₁ → C₂ → Prop) :
+      lts₁.SimulatedBy lts₂ Sim c₁ c₂ →
+      SimilarBy lts₁ lts₂ c₁ c₂
+
+theorem Lts.SimilarBy.refl
+  {lts : Lts C E} {c : C} :
+  Lts.SimilarBy lts lts c c := ⟨
+    λ c₁ c₂ => c₁ = c₂,
+    by simp,
+    by
+      intros c₁ c₂ l c₁' hc₁ hstep
+      subst hc₁
+      exists c₁'
+  ⟩
+
+theorem Lts.SimilarBy.trans
+  {C₁ : Type u₁} {C₂ : Type u₂} {C₃ : Type u₃} {E : Type u₄}
+  {lts₁ : Lts C₁ E} {lts₂ : Lts C₂ E} {lts₃ : Lts C₃ E}
+  {c₁ : C₁} {c₂ : C₂} {c₃ : C₃} :
+  Lts.SimilarBy lts₁ lts₂ c₁ c₂ →
+  Lts.SimilarBy lts₂ lts₃ c₂ c₃ →
+  Lts.SimilarBy lts₁ lts₃ c₁ c₃ := by
+  rintro ⟨R₁₂, hsim₁₂_init, hsim₁₂_coind⟩
+  rintro ⟨R₂₃, hsim₂₃_init, hsim₂₃_coind⟩
+  apply Lts.SimilarBy.mk λ c₁ c₃ => ∃ c₂, R₁₂ c₁ c₂ ∧ R₂₃ c₂ c₃
+  constructor
+  · exists c₂
+  · intros c₁ c₃ l c₁' hR hstep_c₁
+    have ⟨c₂, hR₁₂, hR₂₃⟩ := hR
+    have ⟨c₂', hstep_c₂, hR₁₂'⟩ := hsim₁₂_coind c₁ c₂ l c₁' hR₁₂ hstep_c₁
+    have ⟨c₃', hstep_c₃, hR₂₃'⟩ := hsim₂₃_coind c₂ c₃ l c₂' hR₂₃ hstep_c₂
+    exists c₃'
+    constructor
+    · exact hstep_c₃
+    · exists c₂'
 
 end Wavelet.Lts
