Wavelet/Op.lean
@@ -31,27 +31,19 @@ class InterpConsts (V : Type v) where
   unique_fromBool_toBool : ∀ b, toBool (fromBool b) = some b
   unique_toBool_fromBool : ∀ b v, toBool v = some b → v = fromBool b
 
-/-- The empty operator set -/
-inductive Empty
-
-def Empty.elim {α} (e : Empty) : α := by cases e
-
-instance : Arity Empty where
-  ι e := e.elim
-  ω e := e.elim
-
-inductive Label (Op : Type u) V n [Arity Op] where
+inductive Label (Op : Type u) V m n [Arity Op] where
   | yield (o : Op) (inputs : Vector V (Arity.ι o)) (outputs : Vector V (Arity.ω o))
+  | input (vals : Vector V m)
   | output (vals : Vector V n)
   | τ
 
 /-- A labelled transition with an initial state that can
 interact with uninterpreted operators in `Op` by yielding
 and receiving values of type `V`. -/
-structure Semantics (Op : Type u) (V : Type v) [Arity Op] m n where
+structure Semantics.{u, v, w} (Op : Type u) (V : Type v) [Arity Op] m n : Type (max u v (w + 1)) where
   S : Type w
-  init : Vector V m → S
-  lts : Lts S (Label Op V n)
+  init : S
+  lts : Lts S (Label Op V m n)
 
 /-- Whether the given state can potentially yield. -/
 def Semantics.HasYield
@@ -61,16 +53,37 @@ def Semantics.HasYield
   ∃ outputs s', sem.lts.Step s (.yield op inputs outputs) s'
 
 /-- Simulation modulo the silent label. -/
-abbrev Semantics.Simulates
+abbrev Semantics.SimulatedBy
   [Arity Op]
   (sem₁ sem₂ : Semantics Op V m n)
   (R : sem₁.S → sem₂.S → Prop) : Prop
-  := ∀ args, Lts.Simulates
+  := Lts.SimulatedBy
     (sem₁.lts.StepModTau .τ) (sem₂.lts.StepModTau .τ)
     R
-    (sem₁.init args) (sem₂.init args)
+    sem₁.init sem₂.init
 
-/-- Interprets a set of operators with semantics using another set of operators. -/
+abbrev Semantics.SimilarBy
+  [Arity Op]
+  (sem₁ sem₂ : Semantics Op V m n) : Prop
+  := Lts.SimilarBy sem₁.lts sem₂.lts sem₁.init sem₂.init
+
+infix:50 " ∼ " => Semantics.SimilarBy
+
+theorem Semantics.SimilarBy.refl
+  [Arity Op]
+  (sem : Semantics Op V m n) :
+  sem ∼ sem := Lts.SimilarBy.refl
+
+theorem Semantics.SimilarBy.trans
+  {Op : Type u} {V : Type v}
+  [Arity Op]
+  {sem₁ sem₂ sem₃ : Semantics Op V m n}
+  (h₁ : sem₁ ∼ sem₂) (h₂ : sem₂ ∼ sem₃) :
+  sem₁ ∼ sem₃ :=
+  Lts.SimilarBy.trans h₁ h₂
+
+/-- Interprets a set of operators with semantics using another
+set of operators, with no shared states between them. -/
 abbrev PartInterp Op₀ Op V [Arity Op₀] [Arity Op] :=
   (op : Op) → Semantics Op₀ V (Arity.ι op) (Arity.ω op)
 
@@ -80,16 +93,15 @@ structure Semantics.LinkState
   (main : Semantics (Op₀ ⊕ Op₁) V m n)
   (deps : PartInterp Op₀ Op₁ V) where
   mainState : main.S
-  depStates : (op : Op₁) → Option (deps op).S
+  depStates : (op : Op₁) → (deps op).S
 
 def Semantics.LinkState.init
   [Arity Op₀] [Arity Op₁]
   [DecidableEq Op₁]
   (main : Semantics (Op₀ ⊕ Op₁) V m n)
-  (deps : PartInterp Op₀ Op₁ V)
-  (args : Vector V m) : LinkState main deps := {
-    mainState := main.init args,
-    depStates := λ _ => none,
+  (deps : PartInterp Op₀ Op₁ V) : LinkState main deps := {
+    mainState := main.init,
+    depStates := λ op => (deps op).init ,
   }
 
 inductive Semantics.LinkStep
@@ -97,42 +109,39 @@ inductive Semantics.LinkStep
   [DecidableEq Op₁]
   (main : Semantics (Op₀ ⊕ Op₁) V m n)
   (deps : PartInterp Op₀ Op₁ V)
-  : Lts (LinkState main deps) (Label Op₀ V n) where
+  : Lts (LinkState main deps) (Label Op₀ V m n) where
   | step_main_tau :
     main.lts.Step s.mainState .τ mainState' →
     LinkStep main deps s .τ { s with mainState := mainState' }
   | step_main_yield :
     main.lts.Step s.mainState (.yield (.inl op) inputs outputs) mainState' →
     LinkStep main deps s (.yield op inputs outputs) { s with mainState := mainState' }
+  | step_main_input :
+    main.lts.Step s.mainState (.input inputVals) mainState' →
+    LinkStep main deps s (.input inputVals) { s with mainState := mainState' }
   | step_main_output :
     main.lts.Step s.mainState (.output outputVals) mainState' →
     LinkStep main deps s (.output outputVals) { s with mainState := mainState' }
   | step_dep_tau {depState depState' : (deps depOp).S} :
-    s.depStates depOp = some depState →
-    (deps depOp).lts.Step depState .τ depState' →
+    (deps depOp).lts.Step (s.depStates depOp) .τ depState' →
     LinkStep main deps s .τ
-      { s with depStates := Function.update s.depStates depOp (some depState') }
+      { s with depStates := Function.update s.depStates depOp depState' }
   | step_dep_yield {depState depState' : (deps depOp).S} :
-    s.depStates depOp = some depState →
-    (deps depOp).lts.Step depState (.yield op inputs outputs) depState' →
+    (deps depOp).lts.Step (s.depStates depOp) (.yield op inputs outputs) depState' →
     LinkStep main deps s (.yield op inputs outputs)
-      { s with depStates := Function.update s.depStates depOp (some depState') }
-  -- Semantics to yield and return to the partial interpretation
-  | step_spawn :
+      { s with depStates := Function.update s.depStates depOp depState' }
+  | step_dep_input :
     main.HasYield s.mainState (.inr depOp) inputVals →
-    s.depStates depOp = none → -- No parallel yields to the same dependency
+    (deps depOp).lts.Step (s.depStates depOp) (.input inputVals) depState' →
     LinkStep main deps s .τ
-      { s with depStates :=
-        Function.update s.depStates depOp (some ((deps depOp).init inputVals)) }
-  | step_join
-    {depState : (deps depOp).S} :
-    s.depStates depOp = some depState →
-    (deps depOp).lts.Step depState (.output outputVals) depState' →
+      { s with depStates := Function.update s.depStates depOp depState' }
+  | step_dep_output :
+    (deps depOp).lts.Step (s.depStates depOp) (.output outputVals) depState' →
     main.lts.Step s.mainState (.yield (.inr depOp) inputVals outputVals) mainState' →
     LinkStep main deps s .τ
       { s with
         mainState := mainState',
-        depStates := Function.update s.depStates depOp none }
+        depStates := Function.update s.depStates depOp depState' }
 
 /-- Interprets a subset of operators (`Op₁`) in the remaining ones (`Op₀`). -/
 def Semantics.link
@@ -145,6 +154,61 @@ def Semantics.link
     S := LinkState main deps,
     init := LinkState.init main deps,
     lts := LinkStep main deps,
+  }
+
+/-- The empty operator set -/
+inductive Empty
+
+def Empty.elim {α} (e : Empty) : α := by cases e
+
+instance : Arity Empty where
+  ι e := e.elim
+  ω e := e.elim
+
+/-- Base semantics interprets all of the operators in the same LTS
+with potentially shared states.
+
+TODO: The fact that we need two definitions of semantics (`OpInterp`
+and `Semantics`) is a bit unfortunate. Try unify?
+-/
+class OpInterp (Op : Type u) (V : Type v) [Arity Op] where
+  S : Type w
+  init : S
+  interp :
+    (op : Op) →
+    Vector V (Arity.ι op) → S →
+    Vector V (Arity.ω op) → S → Prop
+
+inductive Semantics.InterpStep
+  [Arity Op]
+  (sem : Semantics Op V m n)
+  (interp : OpInterp Op V)
+  : Lts (sem.S × interp.S) (Label Empty V m n) where
+  | step_tau :
+    sem.lts.Step s .τ s' →
+    InterpStep sem interp (s, t) .τ (s', t)
+  | step_input :
+    sem.lts.Step s (.input inputVals) s' →
+    InterpStep sem interp (s, t) (.input inputVals) (s', t)
+  | step_output :
+    sem.lts.Step s (.output outputVals) s' →
+    InterpStep sem interp (s, t) (.output outputVals) (s', t)
+  | step_yield :
+    sem.lts.Step s (.yield op inputs outputs) s' →
+    interp.interp op inputs t outputs t' →
+    InterpStep sem interp (s, t) .τ (s', t')
+
+/-- Fully interpret all operators using a `OpInterp`
+to get a transition system with only input/output/silent events. -/
+def Semantics.interpret
+  [Arity Op]
+  (sem : Semantics Op V m n)
+  (interp : OpInterp Op V)
+  : Semantics Empty V m n
+  := {
+    S := sem.S × interp.S,
+    init := (sem.init, interp.init),
+    lts := sem.InterpStep interp,
   }
 
 end Wavelet.Op
